---
title: "Monotonicity and
Sandwich Theorem"
description: "Ein Satz"
lead: "Ein Satz"
date: 2020-10-06T08:48:57+00:00
lastmod: 2022-04-01T08:48:57+00:00
draft: false
images: []
menu:
  docs:
    parent: "chapter1"
weight: 100
toc: true
---

## Connections - Overview

{{< header1 "104">}}

## Connections in a table

<details>
<summary><b><u>Show requirements</u></b></summary>
<div class="table-responsive-sm">
<table class="table">
<thead>
  <tr>
    <th scope="col">Concept</th>
    <th scope="col">Content</th>
  </tr>
</thead>
<tbody>

<tr>
<th scope="row"><a href="../../chapter0/000/">Logical Statements
and Operations</a></th>
<td>Logic is the foundation to formulate proofs and to understand the language of mathematics.</td>
</tr>
        
<tr>
<th scope="row"><a href="../../chapter1/101/">Convergence</a></th>
<td>Ein Satz</td>
</tr>
        
<tr>
<th scope="row"><a href="../../chapter1/102/">Boundedness</a></th>
<td>Ein Satz</td>
</tr>
        
</tbody>
</table>
</div>
</details>

<details>
<summary><b><u>Show consequences</u></b></summary>
<div class="table-responsive-sm">
<table class="table">
<thead>
  <tr>
    <th scope="col">Concept</th>
    <th scope="col">Content</th>
  </tr>
</thead>
<tbody>

</tbody>
</table>
</div>
</details>


## Content

{{< tabs tabTotal="4" tabRightAlign="3">}}
{{< tab tabName="Notes" >}}

### Notes 
<div class="Theorem">
<p><span>Monotonicity of limits</span><span id="thm:monseq"
label="thm:monseq"></span> Let <span
class="math inline">\((a_n)_{n\in\mathbb{N}}\)</span> and <span
class="math inline">\((b_n)_{n\in\mathbb{N}}\)</span> be two convergent
real sequences with <span
class="math display">\[\lim_{n\to\infty}a_n=a,\qquad
\lim_{n\to\infty}b_n=b.\]</span> Further, assume that for all <span
class="math inline">\(n\in\mathbb{N}\)</span> holds <span
class="math inline">\(a_n\leq b_n\)</span>. Then the following holds
true:</p>
<ol type="i">
<li><p><span class="math inline">\(a\leq b\)</span>;</p></li>
<li><p>If <span class="math inline">\(a=b\)</span> and <span
class="math inline">\((c_n)_{n\in\mathbb{N}}\)</span> is another
sequence with <span class="math inline">\(a_n\leq c_n\leq b_n\)</span>
for all <span class="math inline">\(n \in \mathbb{N}\)</span>, then
<span class="math inline">\((c_n)_{n\in\mathbb{N}}\)</span> is
convergent with <span
class="math display">\[\lim_{n\to\infty}c_n=a=b.\]</span></p></li>
</ol>
</div>
<div class="proof">
<p><em>Proof.</em></p>
<ol type="i">
<li><p>Consider the sequence of differences between <span
class="math inline">\(b_n\)</span> and <span
class="math inline">\(a_n\)</span>, i.e., <span
class="math inline">\((b_n-a_n)_{n\in\mathbb{N}}\)</span>. By Theorem <a
href="#thm:limformnormed" data-reference-type="ref"
data-reference="thm:limformnormed">[thm:limformnormed]</a>, it suffices
to show that <span
class="math display">\[b-a=\lim_{n\To\infty}(b_n-a_n)\geq0.\]</span>
Assume the converse statement, i.e., <span
class="math inline">\(b-a&lt;0\)</span>. Then, we have that both numbers
<span class="math inline">\(a-b\)</span> and <span
class="math inline">\(b_n-a_n\)</span> are positive and thus <span
class="math display">\[|a-b-(a_n-b_n)|=a-b+(b_n-a_n)&gt;a-b.\]</span> In
particular, there exists no <span
class="math inline">\(n\in\mathbb{N}\)</span> such that <span
class="math inline">\(|a-b-(a_n-b_n)|&lt;\varepsilon\)</span> for <span
class="math inline">\(\varepsilon=a-b&gt;0\)</span>. This is
a contradiction to <span
class="math inline">\(\lim_{n\To\infty}(b_n-a_n)=b-a\)</span>.</p></li>
<li><p>Again consider the sequence <span
class="math inline">\((b_n-a_n)_{n\in\mathbb{N}}\)</span> which is
tending to zero according to Theorem <a href="#thm:limformnormed"
data-reference-type="ref"
data-reference="thm:limformnormed">[thm:limformnormed]</a>. Further,
consider the sequence <span
class="math inline">\((c_n-a_n)_{n\in\mathbb{N}}\)</span>. Then we have
for all <span class="math inline">\(n\in\mathbb{N}\)</span> that <span
class="math inline">\(0\leq c_n-a_n\leq b_n-a_n\)</span>. Let <span
class="math inline">\(\varepsilon&gt;0\)</span>. Since <span
class="math inline">\(b_n-a_n\)</span> is tending to zero, there exists
some <span class="math inline">\(N\)</span> such that for all <span
class="math inline">\(n\geq N\)</span> holds <span
class="math inline">\(|b_n-a_n-0|&lt;\varepsilon\)</span>. Due to <span
class="math inline">\(0\leq c_n-a_n\leq b_n-a_n\)</span>, we can
conclude that for <span class="math inline">\(n\geq N\)</span> holds
<span class="math display">\[|c_n-a_n-0|=c_n-a_n\leq b_n-a_n=
|b_n-a_n-0|&lt;\varepsilon.\]</span> This implies that <span
class="math inline">\((c_n-a_n)_{n\in\mathbb{N}}\)</span> is convergent
with <span class="math inline">\(\lim_{n\to\infty}(c_n-a_n)=0\)</span>.
Hence <span class="math inline">\(a=0+a=\lim_{n\rightarrow\infty}
(c_n-a_n) + \lim_{n\rightarrow\infty} a_n = \lim_{n\rightarrow\infty}
c_n\)</span>.</p></li>
</ol>
<p> ◻</p>
</div>
<div class="Remark">
<p><span id="rem:n_0mon" label="rem:n_0mon"></span> Since the
modification of finitely many sequence elements does not change the
limits (take a closer look at Definition <a href="#def:convlim"
data-reference-type="ref"
data-reference="def:convlim">[def:convlim]</a>), the statements of
Theorem <a href="#thm:monseq" data-reference-type="ref"
data-reference="thm:monseq">[thm:monseq]</a> can be slightly generalised
by only claiming that there exists some <span
class="math inline">\(n_0\)</span> such that for all <span
class="math inline">\(n\geq n_0\)</span> holds <span
class="math inline">\(a_n\leq b_n\)</span> (resp. for all <span
class="math inline">\(n\geq n_0\)</span> holds <span
class="math inline">\(a_n\leq c_n\leq b_n\)</span> in (ii)). In the
proof of (i), one has to replace the words “there exists no <span
class="math inline">\(n\in\mathbb{N}\)</span> such that” by “there
exists no <span class="math inline">\(n\geq n_0\)</span> such that” and
in the proof of (ii) the number <span class="math inline">\(N\)</span>
has to be replaced by <span
class="math inline">\(\max\{N,n_0\}\)</span>.</p>
</div>
<div class="Attention">
<p>From the fact that we have the strict inequality <span
class="math inline">\(a_n&lt;b_n\)</span>, we cannot conclude that the
limits satisfy <span class="math inline">\(a&lt;b\)</span>. To see this,
consider the sequences<span
class="math inline">\((a_n)_{n\in\mathbb{N}}=(0,0,0,\ldots)\)</span> and
<span
class="math inline">\((b_n)_{n\in\mathbb{N}}=(\frac1n)_{n\in\mathbb{N}}\)</span>.
In this case, we have <span class="math inline">\(a=b=0\)</span> though
the strict inequality <span
class="math inline">\(a_n=0&lt;\frac1n=b_n\)</span> holds true for all
<span class="math inline">\(n\in\mathbb{N}\)</span>.</p>
</div>
<div class="example">
<ol type="a">
<li><p>Consider <span
class="math inline">\((\frac1{n^k})_{n\in\mathbb{N}}\)</span> for some
<span class="math inline">\(k\in\mathbb{N}\)</span>. We state two
alternative ways to show that this sequence tends to zero. The first
possibility is, of course, an argumentation as in statement (b) in
Remark on page . The second way to treat this problem is making use of
the inequality <span
class="math display">\[\frac1n\geq\frac1{n^k}&gt;0.\]</span> Since we
know from Example <a href="#ex:basicconvseq" data-reference-type="ref"
data-reference="ex:basicconvseq">[ex:basicconvseq]</a> a) that the
sequence <span class="math inline">\((\frac1n)_{n\in\mathbb{N}}\)</span>
tends to zero, statement (ii) of Theorem <a href="#thm:monseq"
data-reference-type="ref" data-reference="thm:monseq">[thm:monseq]</a>
directly leads to the fact that <span
class="math inline">\((\frac1{n^k})_{n\in\mathbb{N}}\)</span> also tends
to zero.</p></li>
<li><p>Consider <span
class="math inline">\((a_n)_{n\in\mathbb{N}}\)</span> with <span
class="math display">\[a_n=\frac{2n^2+5n-1}{-5n^2+n+1}.\]</span>
Rewriting <span
class="math display">\[a_n=\frac{2+\frac5n-\frac1{n^2}}{-5+\frac1n+\frac1{n^2}},\]</span>
and using that both <span
class="math inline">\((\frac1{n})_{n\in\mathbb{N}}\)</span> and <span
class="math inline">\((\frac1{n^2})_{n\in\mathbb{N}}\)</span> tend to
zero, we can apply Theorem <a href="#thm:limformnormed"
data-reference-type="ref"
data-reference="thm:limformnormed">[thm:limformnormed]</a> to obtain
that <span
class="math display">\[\lim_{n\To\infty}a_n=\lim_{n\To\infty}\frac{2n^2+5n-1}{-5n^2+n+1}=\lim_{n\To\infty}\frac{2+\frac5n-\frac1{n^2}}{-5+\frac1n+\frac1{n^2}}=-\frac25.\]</span></p></li>
<li><p>Consider <span
class="math inline">\((a_n)_{n\in\mathbb{N}}\)</span> with <span
class="math inline">\(a_n=\sqrt{n^2+1}-n\)</span>. At first glance, none
of the so far presented results seem to help to analyse convergence of
this sequence. However, we can compute <span
class="math display">\[\begin{aligned}
a_n\,=&amp;\sqrt{n^2+1}-n
=\frac{(\sqrt{n^2+1}-n)(\sqrt{n^2+1}+n)}{\sqrt{n^2+1}+n}\\
=&amp;\frac{n^2+1-n^2}{\sqrt{n^2+1}+n}
=\frac{1}{\sqrt{n^2+1}+n}&lt;\frac1n.
\end{aligned}\]</span> By Theorem <a href="#thm:monseq"
data-reference-type="ref" data-reference="thm:monseq">[thm:monseq]</a>,
we now get that <span
class="math inline">\(\lim_{n\To\infty}a_n=0\)</span>.</p></li>
</ol>
</div>


{{< /tab >}}
{{< tab tabName="Video" >}}

{{< youtube "Y6rRSip3QN4?start=14">}}

{{< /tab >}}


{{< tab tabName="Podcast">}}
<h3>Podcast</h3>
<h4>Episode 102: Catchy title here</h4>
<audio controls>
  <source src="PODCAST_real" type="audio/wav" />
  Your browser does not support the audio element.
</audio>
<br />
<a href="" class="btn btn-primary btn-lg" download="PODCAST_real"
  >Download</a
>
{{< /tab >}}

{{< tab tabName="Discussion">}}

  <h3>Discussion</h3>
  <h4>Discuss your questions by typing below</h4>

  <iframe
    style="border: 2px solid pink"
    class="embed-responsive-item"
    name="embed_readwrite"
    src="https://pads.rz.tuhh.de/p/"
    width="100%"
    height="600"
  ></iframe>

{{< /tab >}}

{{< /tabs >}}


### WeBWorK Test

{{< webwork "https://demo.webwork.rochester.edu/webwork2/html2xml?&answersSubmitted=0&sourceFilePath=Library/Hope/Calc2/APEX_08_01_Sequences/Q_17.pg&problemSeed=123567890&displayMode=MathJax&courseID=daemon_course&userID=daemon&course_password=daemon&outputformat=simple">}}
