\begin{Theorem}{Formulae for convergent sequences}
\label{thm:limformnormed}
  Let $(a_n)_{n\in\mathbb{N}}$ and $(b_n)_{n\in\mathbb{N}}$ be a~convergent sequences in $\mathbb{K}$. Then the following holds true:
\begin{enumerate}[(i)]
  \item $(a_n+b_n)_{n\in\mathbb{N}}$ is convergent with \[\lim_{n\to\infty}(a_n+b_n)= \lim_{n\to\infty}a_n+\lim_{n\to\infty}b_n.\]
  \item $( a_n\cdot b_n)_{n\in\mathbb{N}}$ is convergent with \[\lim_{n\to\infty}(a_n\cdot b_n)= \lim_{n\to\infty}a_n\cdot\lim_{n\to\infty}b_n.\]
  \item If $\lim_{n\to\infty}b_n\neq0$ and $b_n\neq0$ for all $n\in\mathbb{N}$, then the sequence $(\frac{a_n}{b_n})_{n\in\mathbb{N}}$ is convergent with \[\lim_{n\to\infty}\frac{a_n}{b_n}=\frac{\displaystyle\lim_{n\to\infty}a_n}{\displaystyle\lim_{n\to\infty}b_n}.\]
\end{enumerate}
\end{Theorem}
