\input{packs}

Next we consider sums of convergent series and multiplication of series by some scalar variable. The proof just consists of a~straightforward application of the corresponding Theorems for sequences and is therefore skipped.

\begin{Theorem}[Formulae for convergent series]\label{thm:serlimformnormed}
Let $\lambda\in\mathbb{K}$ and
\[\sum_{k=1}^\infty a_k,\qquad \sum_{k=1}^\infty b_k\]
be two convergent series in $\mathbb{K}$. Then
\begin{enumerate}[(i)]
 \item \[\sum_{k=1}^\infty(a_k+b_k)=\sum_{k=1}^\infty a_k+\sum_{k=1}^\infty b_k;\]
 \item \[\sum_{k=1}^\infty(\lambda a_k)=\lambda \sum_{k=1}^\infty a_k.\]
\end{enumerate}
\end{Theorem}

