\input{packs}

Now we consider rules for the derivatives of sums, products and quotients of functions.
\begin{Theorem}{Summation Rule{,} Product Rule{,} Quotient Rule}
    Let $f,g: I\to\mathbb{R}$ be differentiable in $x_0\in I$.
\begin{enumerate}[(i)]
\item Then $f+g$ is differentiable in $x_0$ with $(f+g)'(x_0)=f'(x_0)+g'(x_0)$.
    %\item for $c\in\mathbb{R}$, $f+g$ is differentiable in $x_0$ with $(f+g)'(x_0)=f'(x_0)+g'(x_0)$;
\item Then $f\cdot g$ is differentiable in $x_0$ with $(f\cdot g)'(x_0)=f'(x_0)\cdot g(x_0)+f(x_0)\cdot g'(x_0)$.
\item If $g(x_0)\neq0$, then $\frac{f}g(x_0)$ is differentiable in $x_0$ with
\[\left(\frac{f}g(x_0)\right)'(x_0)=\frac{f'(x_0)g(x_0)-f(x_0)g'(x_0)}{g^2(x_0)}.\]
\end{enumerate}
\end{Theorem}
{\em Proof:} Let $f(x)=f(x_0)+(x-x_0)\cdot\Delta_{f,x_0}(x)$, $g(x)=g(x_0)+(x-x_0)\cdot\Delta_{g,x_0}(x)$. Then
\begin{enumerate}[(i)]
\item \[(f+g)(x)=f(x)+g(x)=(f+g)(x_0)+(x-x_0)\cdot(\Delta_{f,x_0}(x)+\Delta_{g,x_0}(x)).\]
\item
\[
\begin{aligned}
(f\cdot g)(x)=&
(f(x_0)+(x-x_0)\cdot\Delta_{f,x_0}(x_0))(g(x_0)+(x-x_0)\cdot\Delta_{g,x_0}(x))\\
=&f(x_0)g(x_0)+(x-x_0)(\Delta_{f,x_0}(x_0)g(x_0)+\Delta_{g,x_0}(x)f(x_0))\\&\quad+(x-x_0)^2\Delta_{f,x_0}(x_0)\Delta_{g,x_0}(x)
.\end{aligned}\]
Thus,
\[
\begin{aligned}
&\lim_{x\to x_0}\frac{f(x)g(x)-f(x_0)g(x_0)}{x-x_0}\\
=&\lim_{x\to x_0}\frac{(x-x_0)(\Delta_{f,x_0}(x)g(x_0)+\Delta_{g,x_0}(x)f(x_0))+(x-x_0)^2\Delta_{f,x_0}(x)\Delta_{g,x_0}(x)}{x-x_0}\\
=&\lim_{x\to x_0}\left((\Delta_{f,x_0}(x_0)g(x_0)+\Delta_{g,x_0}(x)f(x_0)+(x-x_0)\Delta_{f,x_0}(x)\Delta_{g,x_0}(x)\right)\\
=&\Delta_{f,x_0}(x)g(x_0)+\Delta_{g,x_0}(x)f(x_0)
\end{aligned}
\]
\item For convenience, we assume that $f\equiv1$ (the general result follows by an application of the product rule). Then
\[\frac1{g(x)}-\frac1{g(x_0)}=\frac{g(x_0)-g(x)}{g(x_0)g(x)}=-\frac{(x-x_0)\Delta_{g,x_0}(x)}{g(x_0)g(x)}\]
and thus
\[\lim_{x\to x_0}\frac1{x-x_0}\left(\frac1{g(x)}-\frac1{g(x_0)}\right)=-\frac{g'(x_0)}{g^2(x_0)}.\]
\end{enumerate}
$\Box$

\begin{example}
\begin{enumerate}[a)]
    \item For a constant $c$ and a~differentiable function $f:I\to\mathbb{R}$ we have
\[(cf)'(x)=c'f(x)+cf'(x)=cf'(x).\]
\item  Let $n\in\mathbb{N}$ and $f:\mathbb{R}\to\mathbb{R}, x\mapsto x^n$. Then $f'(x)=nx^{n-1}$.
\\ Induction basis: $n=1$. $f'(x)=(1\cdot x)'\underset{a)}{=}1=1\cdot x^{1-1}$. \\   
 Induction step: $n>1$: Using the product rule we immediately get
 $$f'(x)=(x^n)'=(x\cdot x^{n-1})' = x'(x^{n-1})+x(x^{n-1})'\underset{\text{Ind. Hyp.}}{=} x^{n-1}+x\cdot (n-1)x^{n-2}=nx^{n-1}$$
\item $f(x)=x^{-n}=\frac1{x^n}$, $n\in\mathbb{N}$. Then for $x\in\mathbb{R}\backslash\{0\}$
\[f'(x)=\frac{-nx^{n-1}}{x^{2n}}=-n\frac{1}{x^{n+1}}=-nx^{-n-1}\]
is true.
\item $f(x)=x\cdot \exp(x)$. Then for $x\in\mathbb{R}$
\[f'(x)=1\cdot\exp(x)+x\cdot\exp(x)=(1+x)\exp(x).\]
\item For a~real polynomial $f(x)=a_nx^n+a_{n-1}x^{n-1}+\ldots+a_1x+a_0$ holds
\[f'(x)=na_nx^{n-1}+(n-1)a_{n-1}x^{n-2}+\ldots+2a_2x+a_1.\]
\end{enumerate}
\end{example}

