\input{packs}

Here, we will prove the theorem below.

\begin{Theorem}{Taylor's formula}
    Let $I$ be an interval and assume that $f:I\to\mathbb{R}$ is $n+1$-times differentiable. Let $x_0\in I$ and $h\in\mathbb{R}$ such that $x_0+h\in I$. 
Then there exists some $\theta\in(0,1)$ such that
\[f(x_0+h)=\underbrace{\sum_{k=0}^n\frac{f^{(k)}(x_0)}{k!}h^k}_{\text{``Taylor polynomial''}}+\underbrace{\frac{f^{(n+1)}(x_0+\theta h)}{(n+1)!}h^{n+1}}_{\text{``remainder term''}}.\]
The number $x_0$ is called \emph{expansion point}.
\end{Theorem}
{\em Proof:} Remember the generalised mean value theorem
\[\frac{F(x_1)-F(x_0)}{g(x_1)-g(x_0)}=\frac{F'(x_0+\theta(x_1-x_0))}{g'(x_0+\theta(x_1-x_0))}\]
for some $\theta\in(0,1)$,
which can be reformulated as (with $h=x_1-x_0$)
\begin{equation}
F(x_0+h)-F(x_0)=\frac{g(x_0+h)-g(x_0)}{g'(x_0+\theta h)}\cdot F'(x_0+\theta h).\label{eq:genmean}
\end{equation}
Now consider the functions
\[F(x):=\sum_{k=0}^n\frac{f^{(k)}(x)}{k!}(x_0+h-x)^k,\qquad g(x):=(x_0+h-x)^{n+1}.\]
Then we have
\[F'(x)=\sum_{k=0}^n\frac{f^{(k+1)}(x)}{k!}(x_0+h-x)^k-\sum_{k=1}^n\frac{f^{(k)}(x)}{(k-1)!}(x_0+h-x)^{k-1}=\frac{f^{(n+1)}(x)}{n!}(x_0+h-x)^{n}.\]
and
\[g'(x)=-(n+1)(x_0+h-x)^{n}.\]
Moreover, we have
\[F(x_0)=\sum_{k=0}^n\frac{f^{(k)}(x_{0})}{k!}h^k,\quad F(x_0+h)=f(x_0+h),\quad g(x_0)=h^{n+1},\quad g(x_0+h)=0.\]
Then using (\ref{eq:genmean}), we obtain
\[
\begin{aligned}
&f(x_0+h)- \sum_{k=0}^n\frac{f^{(k)}(x_0)}{k!}h^k\\
=&F(x_0+h)-F(x_0)\\
=&\frac{g(x_0+h)-g(x_0)}{g'(x_0+\theta h)}\cdot F'(x_0+\theta h)\\
=&\frac{-h^{n+1}}{-(n+1)((1-\theta) h)^{n}}\cdot
\frac{f^{(n+1)}(x_0+\theta h)}{n!}((1-\theta) h)^{n}\\
=&\frac{f^{(n+1)}(x_0+\theta h)}{(n+1)!}h^{n+1}.
\end{aligned}
\]
This implies Taylor's formula.$\Box$

Note that, by the substitution $h:=x-x_0$, Taylor's formula can also be written as follows:
\begin{Theorem}{Taylor's formula{,} alternative version}
    Let $I$ be an interval and assume that $f:I\to\mathbb{R}$ is $n+1$-times differentiable. Let $x_0,x\in I$. Then there exists some $\hat{x}$ between $x_0$ and $x$ 
such that
\[f(x)=\underbrace{\sum_{k=0}^n\frac{f^{(k)}(x_0)}{k!}(x-x_0)^k}_{=:T_n(x,x_0)}+\underbrace{\frac{f^{(n+1)}(\hat{x})}{(n+1)!}(x-x_0)^{n+1}}_{=:R_n(x,x_0)}.\]
\end{Theorem}

